\documentclass{article}
\usepackage[utf8]{inputenc}

\title{Busqueda y ordenaci√≥n 1}
\author{Andoni Latorre Galarraga}
\date{}

\begin{document}

\maketitle

\section{}
$$
t(n) = n + 2 \cdot t(\frac{n}{2}) = n + 2 \cdot ( \frac{n}{2} + 2 \cdot t(\frac{n}{4}) )
$$
$$
= 2 \cdot n + 4 \cdot t(\frac{n}{4}) = 2 \cdot n + 4 \cdot ( \frac{n}{4} + 2 \cdot t(\frac{n}{8}))
$$
$$
= 3 \cdot n + 8 \cdot t(\frac{n}{8}) = \cdots
$$
$$
= k \cdot n + 2^k \cdot t(\frac{n}{2^k})
$$
Cuando $k = \log_2 n$:
$$
t(n) = \log_2 n \cdot n + 2^{\log_2 n} \cdot t(\frac{n}{2^{\log_2 n}})
$$
$$
= n \cdot \log_2 n + n \cdot t(1) = n \cdot \log_2 n + n
$$
\section{}
$$
t(n) = n + t(n-1) = n + n-1 + t(n-2) = n + n-1 + n-2 + t(n-3) =
$$
$$
\cdots = n + n-1 + \cdots + n-k+1 + t(n-k)
$$
Cuando $k = n-1$
$$
= n + n-1 + \cdots + 2 + t(1) = \frac{n^2+n}{2} = \frac{1}{2} n^2 + \frac{1}{2} n
$$
\end{document}